Implement support for quantifiers

byteback-annotations/src/main/java/byteback/annotations/Quantifier.java
@@ -1,53 +1,18 @@
 package byteback.annotations;
 
-import java.util.function.Predicate;
-
 /**
  * Utilities to express quantified expressions.
  */
 public interface Quantifier {
 
-	/**
-	 * Existential quantifier.
-	 * 
-	 * @param d
-	 *            The domain of discourse.
-	 * @param p
-	 *            The predicate applied to the domain.
-	 * @param <T>
-	 *            Type of the iterated elements.
-	 * @return {@code true} if there is a term in {@code d} that satisfies
-	 *         {@code p}.
-	 */
-	public static <T> boolean exists(final Iterable<T> d, final Predicate<T> p) {
-		for (T x : d) {
-			if (p.test(x)) {
-				return true;
-			}
-		}
+  public static int INTEGER = 0;
 
-		return false;
-	}
+	public static boolean exists(int $, boolean p) {
+    return p;
+  }
 
-	/**
-	 * Universal quantifier.
-	 * 
-	 * @param d
-	 *            The domain of discourse.
-	 * @param p
-	 *            The predicate applied to the domain.
-	 * @param <T>
-	 *            Type of the iterated elements.
-	 * @return {@code true} if all terms in {@code d} satisfy {@code p}.
-	 */
-	public static <T> boolean forAll(final Iterable<T> d, final Predicate<T> p) {
-		for (T x : d) {
-			if (!p.test(x)) {
-				return false;
-			}
-		}
-
-		return true;
+	public static boolean forall(int $, boolean p) {
+		return p;
 	}
 
 }
