byteback-core/src/integration/java/byteback/core/converter/soottoboogie/FunctionConverterIntegrationTest.java
@@ -45,8 +45,9 @@ public class FunctionConverterIntegrationTest extends ConverterFixture {
 	}
 
 	@Test
-	public void Convert_GivenRegressionSet_ReturnsExpectedCode() {
-		assertEquals(PrintUtil.toString(parameter.expected), PrintUtil.toString(parameter.actual));
+  public void Convert_GivenRegressionSet_ReturnsExpectedCode() {
+    System.out.println(PrintUtil.toString(parameter.actual));
+    assertEquals(PrintUtil.toString(parameter.expected), PrintUtil.toString(parameter.actual));
 	}
 
 }
