byteback-core/src/main/java/byteback/core/converter/soottoboogie/field/FieldConverter.java
@@ -5,9 +5,8 @@ import byteback.core.converter.soottoboogie.Prelude;
 import byteback.core.converter.soottoboogie.type.TypeAccessExtractor;
 import byteback.core.representation.soot.unit.SootField;
 import byteback.frontend.boogie.ast.ConstantDeclaration;
-import byteback.frontend.boogie.ast.Declarator;
-import byteback.frontend.boogie.ast.SetBinding;
 import byteback.frontend.boogie.ast.TypeAccess;
+import byteback.frontend.boogie.builder.SetBindingBuilder;
 
 public class FieldConverter {
 
@@ -19,12 +18,12 @@ public class FieldConverter {
 
 	public ConstantDeclaration convert(final SootField field) {
 		final ConstantDeclaration constantDeclaration = new ConstantDeclaration();
-		final SetBinding binding = new SetBinding();
+		final var bindingBuilder = new SetBindingBuilder();
 		final TypeAccess baseTypeAccess = new TypeAccessExtractor().visit(field.getType());
 		final TypeAccess fieldTypeAccess = Prelude.getFieldTypeAccess(baseTypeAccess);
-		constantDeclaration.setBinding(binding);
-		binding.setTypeAccess(fieldTypeAccess);
-		binding.addDeclarator(new Declarator(NameConverter.fieldName(field)));
+		bindingBuilder.typeAccess(fieldTypeAccess);
+		bindingBuilder.name(NameConverter.fieldName(field));
+		constantDeclaration.setBinding(bindingBuilder.build());
 
 		return constantDeclaration;
 	}
