byteback-core/src/main/java/byteback/core/converter/soottoboogie/function/FunctionBodyExtractor.java
@@ -1,10 +1,9 @@
 package byteback.core.converter.soottoboogie.function;
 
+import byteback.core.converter.soottoboogie.LocalExtractor;
 import byteback.core.converter.soottoboogie.LocalUseExtractor;
-import byteback.core.converter.soottoboogie.expression.SubstitutingExtractor;
 import byteback.core.converter.soottoboogie.expression.Substitutor;
 import byteback.core.representation.soot.body.SootExpression;
-import byteback.core.representation.soot.body.SootExpressionVisitor;
 import byteback.core.representation.soot.body.SootStatementVisitor;
 import byteback.core.representation.soot.type.SootType;
 import byteback.core.util.CountingMap;
@@ -17,31 +16,6 @@ import soot.*;
 import soot.jimple.*;
 
 public class FunctionBodyExtractor extends SootStatementVisitor<Expression> {
-
-  public static class LocalExtractor extends SootExpressionVisitor<Local> {
-
-    private Local local;
-
-    @Override
-    public void caseLocal(final Local local) {
-      this.local = local;
-    }
-
-    @Override
-    public void caseDefault(final Value expression) {
-      throw new IllegalArgumentException("Expected local definition, got " + expression);
-    }
-
-    @Override
-    public Local result() {
-      if (local == null) {
-        throw new IllegalStateException("Could not retrieve local reference");
-      } else {
-        return local;
-      }
-    }
-
-  }
 
   private static final Logger log = LoggerFactory.getLogger(FunctionBodyExtractor.class);
 
@@ -64,14 +38,16 @@ public class FunctionBodyExtractor extends SootStatementVisitor<Expression> {
     final var left = new SootExpression(assignment.getLeftOp());
     final var right = new SootExpression(assignment.getRightOp());
     final Local local = new LocalExtractor().visit(left);
-    final Expression boogieExpression = new SubstitutingExtractor(substitutor).visit(right, left.getType());
+    final Expression boogieExpression = new FunctionExpressionExtractor(substitutor)
+      .visit(right, left.getType());
     substitutor.put(local, new LocalUseExtractor().visit(right), boogieExpression);
   }
 
   @Override
   public void caseReturnStmt(final ReturnStmt returnStatement) {
     final var operand = new SootExpression(returnStatement.getOp());
-    result = new SubstitutingExtractor(substitutor).visit(operand, returnType);
+    result = new FunctionExpressionExtractor(substitutor)
+      .visit(operand, returnType);
 
     for (Entry<Local, Integer> entry : expressionTable.getAccessCount().entrySet()) {
       if (entry.getValue() == 0) {
