byteback-core/src/main/java/byteback/core/converter/soottoboogie/function/FunctionExpressionExtractor.java
@@ -1,0 +1,71 @@
+package byteback.core.converter.soottoboogie.function;
+
+import java.util.Iterator;
+
+import byteback.core.converter.soottoboogie.Annotations;
+import byteback.core.converter.soottoboogie.LocalExtractor;
+import byteback.core.converter.soottoboogie.expression.SubstitutingExtractor;
+import byteback.core.converter.soottoboogie.expression.Substitutor;
+import byteback.core.converter.soottoboogie.type.TypeAccessExtractor;
+import byteback.core.representation.soot.body.SootExpression;
+import byteback.core.representation.soot.type.SootType;
+import byteback.core.representation.soot.unit.SootMethod;
+import byteback.frontend.boogie.ast.ExistentialQuantifier;
+import byteback.frontend.boogie.ast.Quantifier;
+import byteback.frontend.boogie.ast.UniversalQuantifier;
+import byteback.frontend.boogie.builder.QuantifierExpressionBuilder;
+import byteback.frontend.boogie.builder.SetBindingBuilder;
+import soot.BooleanType;
+import soot.Local;
+
+public class FunctionExpressionExtractor extends SubstitutingExtractor {
+
+  public FunctionExpressionExtractor(final Substitutor substitutor) {
+    super(substitutor);
+  }
+
+  public void pushQuantifier(final Quantifier quantifier, final Iterable<SootExpression> arguments) {
+    final var quantifierBuilder = new QuantifierExpressionBuilder();
+    final var bindingBuilder = new SetBindingBuilder();
+    final Iterator<SootExpression> argumentsIterator = arguments.iterator();
+    final Local variableLocal = new LocalExtractor().visit(argumentsIterator.next());
+    bindingBuilder.typeAccess(new TypeAccessExtractor().visit(new SootType(variableLocal.getType())));
+    bindingBuilder.name(variableLocal.getName());
+    quantifierBuilder.quantifier(quantifier);
+    quantifierBuilder.addBinding(bindingBuilder.build());
+    quantifierBuilder.operand(visit(argumentsIterator.next(), new SootType(BooleanType.v())));
+    pushExpression(quantifierBuilder.build());
+  }
+
+  public void pushExistentialQuantifier(Iterable<SootExpression> arguments) {
+    final Quantifier quantifier = ExistentialQuantifier.instance();
+    pushQuantifier(quantifier, arguments);
+  }
+
+  public void pushUniversalQuantifier(final Iterable<SootExpression> arguments) {
+    final Quantifier quantifier = UniversalQuantifier.instance();
+    pushQuantifier(quantifier, arguments);
+  }
+
+  public void pushQuantifier(final SootMethod method, final Iterable<SootExpression> arguments) {
+    final String quantifierName = method.getName();
+
+    if (quantifierName.equals(Annotations.EXISTENTIAL_QUANTIFIER_NAME)) {
+      pushExistentialQuantifier(arguments);
+    } else if (quantifierName.equals(Annotations.UNIVERSAL_QUANTIFIER_NAME)) {
+      pushUniversalQuantifier(arguments);
+    } else {
+			throw new RuntimeException("Unknown quantifier method: " + method.getName());
+    }
+  }
+
+  @Override
+  public void pushFunctionReference(final SootMethod method, final Iterable<SootExpression> arguments) {
+    if (method.getSootClass().equals(Annotations.QUANTIFIER_CLASS)) {
+      pushQuantifier(method, arguments);
+    } else {
+      super.pushFunctionReference(method, arguments);
+    }
+  }
+
+}
