byteback-dummy/java8/src/main/java/byteback/dummy/function/Simple.java
@@ -1,0 +1,26 @@
+package byteback.dummy.function;
+
+import byteback.annotations.Contract.Pure;
+import static byteback.annotations.Quantifier.forall;
+
+import byteback.annotations.Quantifier;
+
+import static byteback.annotations.Quantifier.exists;
+
+public class Simple {
+
+  @Pure
+  public static boolean universalQuantifier() {
+    int i = Quantifier.INTEGER;
+
+    return forall(i, true);
+  }
+
+  @Pure
+  public static boolean existentialQuantifier() {
+    int i = Quantifier.INTEGER;
+
+    return exists(i, true);
+  }
+
+}
