byteback-core/src/integration/resources/regression/java8/boogie/byteback.dummy.function.Boolean.bpl
@@ -8,17 +8,17 @@ function byteback.dummy.function.Boolean.and#boolean#boolean#(~heap: Store, a: b
     a && b
 }
 
-function byteback.dummy.function.Boolean.xor#boolean#boolean#(~heap: Store, a: bool, b: bool) returns(bool)
+function byteback.dummy.function.Boolean.xor#boolean#boolean#(~heap: Store, a: bool, b: bool) returns (bool)
 {
     a != b
 }
 
-function byteback.dummy.function.Boolean.returnsTrue##(~heap: Store) returns(bool)
+function byteback.dummy.function.Boolean.returnsTrue##(~heap: Store) returns (bool)
 {
     true
 }
 
-function byteback.dummy.function.Boolean.returnsFalse##(~heap: Store) returns(bool)
+function byteback.dummy.function.Boolean.returnsFalse##(~heap: Store) returns (bool)
 {
     false
 }
