byteback-core/src/integration/resources/regression/java8/boogie/byteback.dummy.function.Simple.bpl
@@ -1,0 +1,9 @@
+function byteback.dummy.function.Simple.universalQuantifier##(~heap: Store) returns (bool)
+{
+  (forall i : int :: true)
+}
+
+function byteback.dummy.function.Simple.existentialQuantifier##(~heap: Store) returns (bool)
+{
+  (exists i : int :: true)
+}
